nola/examples/logic/deriv.v
@@ -5,13 +5,13 @@ From iris.proofmode Require Export proofmode.
 
 (** ** [nderivsi]: [derivsi] for [nPropL] *)
 Definition nderivsi Σ `{!nintpGS Σ} : derivsi :=
-  Intpsi (nderivs Σ) (λ d '(Darg _ P), ⟦ P ⟧(d)).
+  Derivsi (nderivs Σ) (λ d '(Darg _ P), ⟦ P ⟧(d)).
 
 (** Notation for [nderivsi] *)
 Notation nderivy Σ := (derivy (nderivsi Σ)).
-Notation nderiv := (deriv (ITI:=nderivsi _)).
-Notation ndsound d := (dsound (ITI:=nderivsi _) d ()).
-Notation nderiv_sound := (deriv_sound (ITI:=nderivsi _)).
+Notation nderiv := (deriv (DI:=nderivsi _)).
+Notation ndsound d := (dsound (DI:=nderivsi _) d ()).
+Notation nderiv_sound := (deriv_sound (DI:=nderivsi _)).
 
 (** Utility for [nderiv] *)
 Notation nninvd := (nninv nderiv).
